src/verso-manual/VersoManual.lean
@@ -433,11 +433,6 @@ def emitSearchIndex (dir : System.FilePath) (state : TraverseState) (logError : 
   | .error e => logError e
   | .ok index =>
     let indexJs := "const searchIndex_ = " ++ index.toJson.compress ++ ";\n\n"
-    -- let .ok xs := Verso.Search.mkIndexDocs doc
-    --   | panic! "nope"
-    -- let indexJsExtra :=
-    --   "const searchIndex2 = elasticlunr(function() { this.addField('id'); this.addField('contents');} );\n" ++
-    --   xs.foldl (init := "") fun js doc => js ++ "searchIndex2.addDoc({'id':" ++ doc.id.quote ++ ",'contents':"++ doc.content.quote ++ "});\n"
     let indexJs := indexJs ++ "const searchIndex = elasticlunr ? elasticlunr.Index.load(searchIndex_) : null;\n"
     let indexJs := indexJs ++ "window.searchIndex = elasticlunr ? searchIndex : null;\n"
     IO.FS.writeFile (dir / "searchIndex.js") <| indexJs
